src/UntypedComp6.v
@@ -1,0 +1,677 @@
+Require Import Common.
+
+Require Import Utopia.
+Require Import Metadata.
+Require Import Program.
+
+Require Import ListLemmas.
+Require Import Monads.
+Require Import HList.
+Require Import CompilationUnit.
+Require Import Semantics.
+Require Import HighestValues.
+
+Require Untyped4.
+Require Untyped5.
+Require Untyped6.
+
+Module A := Untyped5.
+Module S := Untyped4.
+Module B := Untyped6.
+
+
+Definition compile_genv := @id (list S.expr).
+
+Inductive I_expr : S.expr -> S.expr -> Prop :=
+| IValue : forall av bv,
+        B.expr_value bv av ->
+        I_expr (S.Value av) bv
+| IArg : I_expr (S.Arg) (S.Arg)
+| IUpVar : forall idx, I_expr (S.UpVar idx) (S.UpVar idx)
+| IApp : forall af aa bf ba,
+        I_expr af bf ->
+        I_expr aa ba ->
+        I_expr (S.App af aa) (S.App bf ba)
+| IMkConstr : forall ctor aargs bargs,
+        Forall2 I_expr aargs bargs ->
+        I_expr (S.MkConstr ctor aargs) (S.MkConstr ctor bargs)
+| IMkClose : forall fname afree bfree,
+        Forall2 I_expr afree bfree ->
+        I_expr (S.MkClose fname afree) (S.MkClose fname bfree)
+| IElim : forall ty acases atarget bcases btarget,
+        Forall2 I_expr acases bcases ->
+        I_expr atarget btarget ->
+        I_expr (S.Elim ty acases atarget) (S.Elim ty bcases btarget)
+.
+
+Inductive I_cont : S.cont -> S.cont -> Prop :=
+| IKAppL : forall ae2 l ak  be2 bk,
+        I_expr ae2 be2 ->
+        I_cont ak bk ->
+        I_cont (S.KAppL ae2 l ak) (S.KAppL be2 l bk)
+| IKAppR : forall ae1 l ak  be1 bk,
+        I_expr ae1 be1 ->
+        I_cont ak bk ->
+        I_cont (S.KAppR ae1 l ak) (S.KAppR be1 l bk)
+| IKConstr : forall ctor  avs aes l ak  bvs bes bk,
+        Forall2 I_expr avs bvs ->
+        Forall2 I_expr aes bes ->
+        I_cont ak bk ->
+        I_cont (S.KConstr ctor avs aes l ak)
+               (S.KConstr ctor bvs bes l bk)
+| IKClose : forall fname  avs aes l ak  bvs bes bk,
+        Forall2 I_expr avs bvs ->
+        Forall2 I_expr aes bes ->
+        I_cont ak bk ->
+        I_cont (S.KClose fname avs aes l ak)
+               (S.KClose fname bvs bes l bk)
+| IKElim : forall ty  acases l ak  bcases bk,
+        Forall2 I_expr acases bcases ->
+        I_cont ak bk ->
+        I_cont (S.KElim ty acases l ak)
+               (S.KElim ty bcases l bk)
+.
+
+Fixpoint unroll_cont e depth k :=
+    match depth with
+    | 0 => Some e
+    | S depth =>
+            match k with
+            | S.KConstr ctor vs es _ k =>
+                    let e' := S.MkConstr ctor (vs ++ e :: es) in
+                    unroll_cont e' depth k
+            | S.KClose fname vs es _ k => 
+                    let e' := S.MkClose fname (vs ++ e :: es) in
+                    unroll_cont e' depth k
+            | _ => None
+            end
+    end.
+
+Fixpoint drop_cont depth k :=
+    match depth with
+    | 0 => Some k
+    | S depth =>
+            match k with
+            | S.KConstr _ _ _ _ k => drop_cont depth k
+            | S.KClose _ _ _ _ k => drop_cont depth k
+            | _ => None
+            end
+    end.
+
+Fixpoint locals_match l depth k :=
+    match depth with
+    | 0 => True
+    | S depth =>
+            match k with
+            | S.KConstr _ _ _ l' k => l' = l /\ locals_match l depth k
+            | S.KClose _ _ _ l' k => l' = l /\ locals_match l depth k
+            | _ => False
+            end
+    end.
+
+Inductive I : S.state -> S.state -> Prop :=
+| IRun : forall ae l ak  be bk,
+        I_expr ae be ->
+        I_cont ak bk ->
+        I (S.Run ae l ak) (S.Run be l bk)
+
+| IInValue : forall l v (apat bpat : S.expr -> S.expr) depth,
+        (* `x_cur`: the `x` in the current state. *)
+        (* `x_last`: the last `x` we'll see before returning to  an `IRun` state. *)
+        forall ae_cur ae_last ak_cur ak_last ak,
+        forall be_last bk,
+
+        unroll_cont ae_cur depth ak_cur = Some ae_last ->
+        drop_cont depth ak_cur = Some ak_last ->
+        locals_match l depth ak_cur ->
+
+        B.expr_value ae_last v ->
+        B.expr_value be_last v ->
+
+        (forall a b, I_expr a b -> I_expr (apat a) (bpat b)) ->
+        S.run_cont ak_last v = S.Run (apat (S.Value v)) l ak ->
+        I_cont ak bk ->
+
+        I (S.Run ae_cur l ak_cur) (S.Run (bpat be_last) l bk)
+
+| IStop : forall v,
+        I (S.Stop v) (S.Stop v)
+.
+
+
+
+Ltac i_ctor := intros; constructor; eauto.
+Ltac i_lem H := intros; eapply H; eauto.
+
+Lemma I_run_cont : forall v ak bk,
+    I_cont ak bk ->
+    I (S.run_cont ak v) (S.run_cont bk v).
+intros0 II; invc II; repeat i_ctor.
+- i_lem Forall2_app. i_ctor. i_ctor. i_ctor.
+- i_lem Forall2_app. i_ctor. i_ctor. i_ctor.
+Qed.
+
+(*
+Lemma I_value_value : forall a b,
+    I_value a b ->
+    B.value b.
+mut_induction a using value_rect_mut' with
+    (Pl := fun as_ => forall bs,
+        Forall2 I_value as_ bs ->
+        Forall B.value bs);
+[ intros0 II; invc II; simpl; repeat i_ctor.. | ].
+finish_mut_induction I_value_value using list.
+Qed exporting.
+Hint Resolve I_value_value.
+Hint Resolve I_value_value_list.
+*)
+
+Lemma I_is_value : forall a b,
+    I_expr a b ->
+    S.is_value a ->
+    B.is_value b.
+intros0 II Aval; invc Aval; invc II; eexists; eauto.
+Qed.
+Hint Resolve I_is_value.
+
+Lemma I_expr_refl : forall e,
+    I_expr e e.
+mut_induction e using S.expr_rect_mut' with
+    (Pl := fun es => Forall2 I_expr es es);
+[ i_ctor.. | ].
+- i_ctor.
+- finish_mut_induction I_expr_refl using list.
+Qed exporting.
+Hint Resolve I_expr_refl.
+Hint Resolve I_expr_refl_list.
+
+(*
+Lemma I_isnt_value : forall a b,
+    I_expr a b ->
+    ~ AS.is_value a ->
+    ~ B.value b.
+intros0 II Hval; contradict Hval; invc Hval; invc II. on >I_value, invc; i_ctor.
+Qed.
+Hint Resolve I_isnt_value.
+
+Lemma I_expr_map_value : forall vs bes,
+    Forall2 I_expr (map AS.Value vs) bes ->
+    bes = map B.Value vs.
+induction vs; destruct bes; intros0 II; invc II; simpl.
+- reflexivity.
+- on (I_expr _ _), invc.
+  f_equal. i_lem IHvs.
+Qed.
+*)
+
+
+Lemma I_unroll_elim' : forall acase bcase ctor args amk_rec bmk_rec idx,
+    I_expr acase bcase ->
+    (forall a b, I_expr a b -> I_expr (amk_rec a) (bmk_rec b)) ->
+    I_expr (S.unroll_elim' acase ctor args amk_rec idx)
+           (S.unroll_elim' bcase ctor args bmk_rec idx).
+first_induction args; intros0 IIcase IImk_rec; simpl.
+- assumption.
+- break_if.
+  + eapply IHargs; eauto. repeat i_ctor.
+  + eapply IHargs; eauto. repeat i_ctor.
+Qed.
+
+Lemma I_unroll_elim : forall acase bcase ctor args amk_rec bmk_rec,
+    I_expr acase bcase ->
+    (forall a b, I_expr a b -> I_expr (amk_rec a) (bmk_rec b)) ->
+    I_expr (S.unroll_elim acase ctor args amk_rec)
+           (S.unroll_elim bcase ctor args bmk_rec).
+intros. eapply I_unroll_elim'; auto.
+Qed.
+
+
+Lemma expr_value_inj : forall e v v',
+    B.expr_value e v ->
+    B.expr_value e v' ->
+    v = v'.
+mut_induction e using S.expr_rect_mut' with
+    (Pl := fun es => forall vs vs',
+        Forall2 B.expr_value es vs ->
+        Forall2 B.expr_value es vs' ->
+        vs = vs');
+[ intros0 Hv Hv'; invc Hv; invc Hv'.. | ].
+
+- reflexivity.
+- replace args_v with args_v0 by (eapply IHe; eauto). reflexivity.
+- replace free_v with free_v0 by (eapply IHe; eauto). reflexivity.
+
+- reflexivity.
+- replace y with y0 by eauto.
+  replace l' with l'0 by eauto.
+  reflexivity.
+
+- finish_mut_induction expr_value_inj using list.
+Qed exporting.
+
+Lemma expr_value_eq : forall v v',
+    B.expr_value (S.Value v) v' ->
+    v' = v.
+mut_induction v using value_rect_mut' with
+    (Pl := fun vs => forall vs',
+        Forall2 B.expr_value (map S.Value vs) vs' ->
+        vs' = vs);
+[ intros0 Hev; invc Hev; eauto.. | ].
+
+- rewrite (IHv _ **). rewrite (IHv0 ?? **). reflexivity.
+
+- finish_mut_induction expr_value_eq using list.
+Qed exporting.
+
+Lemma I_expr_expr_value : forall a b v,
+    I_expr a b ->
+    B.expr_value b v ->
+    B.expr_value a v.
+mut_induction a using S.expr_rect_mut' with
+    (Pl := fun as_ => forall bs vs,
+        Forall2 I_expr as_ bs ->
+        Forall2 B.expr_value bs vs ->
+        Forall2 B.expr_value as_ vs);
+[ intros0 II Hev; invc Hev; invc II.. | ].
+
+- on >B.expr_value, invc. i_ctor.
+
+- on >B.expr_value, invc.
+  replace args_v0 with args_v by eauto using expr_value_inj_list.
+  i_ctor.
+
+- on >B.expr_value, invc.
+  replace free_v0 with free_v by eauto using expr_value_inj_list.
+  i_ctor.
+
+- i_ctor.
+
+- i_ctor.
+
+- i_ctor.
+- i_ctor.
+
+- finish_mut_induction I_expr_expr_value using list.
+Qed exporting.
+
+Lemma I_expr_expr_value' : forall b v,
+    I_expr (S.Value v) b ->
+    B.expr_value b v.
+mut_induction b using S.expr_rect_mut' with
+    (Pl := fun bs => forall vs,
+        Forall2 (fun v b => I_expr (S.Value v) b) vs bs ->
+        Forall2 B.expr_value bs vs);
+[ intros0 II; invc II; try on >B.expr_value, invc; try i_ctor.. | ].
+- finish_mut_induction I_expr_expr_value' using list.
+Qed exporting.
+
+Lemma I_expr_value : forall a b,
+    I_expr a b ->
+    S.is_value a ->
+    B.is_value b.
+mut_induction a using S.expr_rect_mut' with
+    (Pl := fun as_ => forall bs,
+        Forall2 I_expr as_ bs ->
+        Forall S.is_value as_ ->
+        Forall B.is_value bs);
+[ intros0 II Aval; invc Aval; invc II; try i_ctor.. | ].
+- eexists. eauto.
+- finish_mut_induction I_expr_value using list.
+Qed exporting.
+Hint Resolve I_expr_value.
+Hint Resolve I_expr_value_list.
+
+
+
+Lemma unroll_cont_not_value : forall e e' depth k,
+    (forall v, ~ B.expr_value e v) ->
+    unroll_cont e depth k = Some e' ->
+    (forall v, ~ B.expr_value e' v).
+first_induction depth; intros0 Hnval Hunroll; intros.
+- simpl in *. inject_some. auto.
+
+- destruct k; simpl in *; try discriminate.
+
+  + eapply IHdepth; [ | eassumption ]. intros. inversion 1.
+    on >Forall2, invc_using Forall2_app_inv.
+    on >Forall2, invc.
+    eapply Hnval. eauto.
+
+  + eapply IHdepth; [ | eassumption ]. intros. inversion 1.
+    on >Forall2, invc_using Forall2_app_inv.
+    on >Forall2, invc.
+    eapply Hnval. eauto.
+Qed.
+
+Lemma unroll_cont_ex : forall e e' depth k result,
+    unroll_cont e depth k = Some result ->
+    exists result', unroll_cont e' depth k = Some result'.
+first_induction depth; intros0 Hcont; simpl in *.
+- eauto.
+- destruct k; try discriminate; eauto.
+Qed.
+
+Lemma unroll_cont_I_expr : forall e e' depth k result result',
+    unroll_cont e depth k = Some result ->
+    unroll_cont e' depth k = Some result' ->
+    I_expr e e' ->
+    I_expr result result'.
+first_induction depth; intros0 Hcont Hcont' II; simpl in *.
+- inject_some. auto.
+- destruct k; try discriminate; eauto.
+  + i_lem IHdepth. i_ctor. i_lem Forall2_app.
+  + i_lem IHdepth. i_ctor. i_lem Forall2_app.
+Qed.
+
+Lemma unroll_cont_expr_value : forall e e' depth k result result' v,
+    unroll_cont e depth k = Some result ->
+    unroll_cont e' depth k = Some result' ->
+    (forall v', B.expr_value e v' -> B.expr_value e' v') ->
+    B.expr_value result v ->
+    B.expr_value result' v.
+first_induction depth; intros0 Hcont Hcont' Hev Hresult; simpl in *.
+- inject_some. auto.
+- destruct k; try discriminate; eauto.
+  all: eapply IHdepth with (1 := Hcont) (2 := Hcont'); eauto.
+  all: intros; on >B.expr_value, invc; i_ctor.
+  all: on >Forall2, invc_using Forall2_app_inv; i_lem Forall2_app.
+  all: on >Forall2, invc; i_ctor.
+Qed.
+
+Lemma MkConstr_expr_value : forall ctor vs e e' es,
+    (forall v', B.expr_value e v' -> B.expr_value e' v') ->
+    forall v,
+    B.expr_value (S.MkConstr ctor (vs ++ e :: es)) v ->
+    B.expr_value (S.MkConstr ctor (vs ++ e' :: es)) v.
+intros0 Hev. intros.
+on >B.expr_value, invc.  i_ctor.
+on >Forall2, invc_using Forall2_app_inv.  i_lem Forall2_app.
+on >Forall2, invc.  i_ctor.
+Qed.
+
+Lemma MkClose_expr_value : forall fname vs e e' es,
+    (forall v', B.expr_value e v' -> B.expr_value e' v') ->
+    forall v,
+    B.expr_value (S.MkClose fname (vs ++ e :: es)) v ->
+    B.expr_value (S.MkClose fname (vs ++ e' :: es)) v.
+intros0 Hev. intros.
+on >B.expr_value, invc.  i_ctor.
+on >Forall2, invc_using Forall2_app_inv.  i_lem Forall2_app.
+on >Forall2, invc.  i_ctor.
+Qed.
+
+Lemma MkConstr_expr_value_2 : forall ctor vs v,
+    B.expr_value (S.MkConstr ctor (map S.Value vs)) v ->
+    B.expr_value (S.Value (Constr ctor vs)) v.
+intros.
+on >B.expr_value, invc.
+replace args_v with vs in * by (symmetry; eauto using expr_value_eq_list).
+i_ctor.
+Qed.
+
+Lemma MkClose_expr_value_2 : forall fname vs v,
+    B.expr_value (S.MkClose fname (map S.Value vs)) v ->
+    B.expr_value (S.Value (Close fname vs)) v.
+intros.
+on >B.expr_value, invc.
+replace free_v with vs in * by (symmetry; eauto using expr_value_eq_list).
+i_ctor.
+Qed.
+
+
+
+
+
+
+
+Definition metric (s : S.state) := 0.
+
+Theorem I_sim : forall AE BE a a' b,
+    Forall2 I_expr AE BE ->
+    I a b ->
+    A.sstep AE a a' ->
+    exists b',
+        (B.sstep BE b b' \/ (b' = b /\ metric a' < metric a)) /\
+        I a' b'.
+destruct a as [ae l ak | v];
+intros0 Henv II Astep; inv Astep.
+all: invc II.
+(* Not sure why, but  the `fwd eapply` breaks if it's after the `invc I_expr`... *)
+(* all: try (fwd eapply Forall2_nth_error_ex as HH; eauto; [ ]). *)
+all: try on (I_expr _ be), invc.
+
+all: try solve [
+    on (B.expr_value ae_last _), contradict;
+    eapply unroll_cont_not_value; [ | eassumption ];
+    inversion 1
+    ].
+
+(* SValue *)
+- on >B.expr_value, invc.
+  + eexists. split. left. i_lem B.SValue.
+    i_lem I_run_cont.
+  + eexists. split. left. i_lem B.SConstrDone.
+    i_ctor. i_lem I_run_cont.
+  + eexists. split. left. i_lem B.SCloseDone.
+    i_ctor. i_lem I_run_cont.
+
+(* SValue - IInValue *)
+- destruct depth as [ | depth' ].
+
+  + (* Depth is zero.  Left pops a continuation, returning to correspondence
+       with the right. *)
+    simpl in *.
+    inject_some.
+    on (B.expr_value (S.Value _) _), invc.
+    on (S.run_cont _ _ = _), fun H => (rewrite H; clear H).
+
+    eexists. split. right. split. reflexivity.
+    * admit. (* metric *)
+    * i_ctor. on _, eapply_. i_ctor.
+
+  + (* Depth is nonzero.  Left pops a continuation and remains in IInValue. *)
+    destruct ak; try discriminate; simpl in *.
+
+    * eexists. split. right. split. reflexivity.
+      -- admit. (* metric *)
+      -- break_and. subst l0. i_lem IInValue.
+    * eexists. split. right. split. reflexivity.
+      -- admit. (* metric *)
+      -- break_and. subst l0. i_lem IInValue.
+
+
+(* SArg *)
+- eexists. split. left. i_lem B.SArg.
+  i_lem I_run_cont.
+
+(* SUpVar *)
+- eexists. split. left. i_lem B.SUpVar.
+  i_lem I_run_cont.
+
+
+(* SAppL *)
+- destruct (B.value_dec bf) as [[bf_v ?] | ?].
+
+  + (* Right is already a value, but left needs to do work.  Step to IInValue. *)
+    eexists. split. right. split. reflexivity.
+    * admit. (* metric *)
+    * eapply IInValue with (depth := 0)
+        (apat := fun f => S.App f _) (bpat := fun f => S.App f _);
+        simpl; eauto using I_expr_expr_value.
+      -- i_ctor.
+      -- reflexivity.
+
+  + (* Left and right are both values.  Proceed in lockstep. *)
+    eexists. split. left. i_lem B.SAppL.
+    i_ctor. i_ctor.
+
+(* SAppR *)
+- destruct (B.value_dec ba) as [[ba_v ?] | ?].
+
+  + (* Right is already a value, but left needs to do work.  Step to IInValue. *)
+    eexists. split. right. split. reflexivity.
+    * admit. (* metric *)
+    * eapply IInValue with (depth := 0)
+        (apat := fun a => S.App _ a) (bpat := fun a => S.App _ a);
+        simpl; eauto using I_expr_expr_value.
+      -- i_ctor.
+      -- reflexivity.
+
+  + (* Left and right are both values.  Proceed in lockstep. *)
+    eexists. split. left. i_lem B.SAppR.
+    i_ctor. i_ctor.
+
+(* SMakeCall *)
+- fwd eapply Forall2_nth_error_ex as HH; eauto.  destruct HH as (bbody & ? & ?).
+  eexists. split. left. i_lem B.SMakeCall.
+  + i_lem I_expr_expr_value'.
+  + i_lem I_expr_expr_value'.
+  + i_ctor.
+
+
+(* SConstrStep *)
+- on _, invc_using Forall2_3part_inv.
+  rename ys1 into bvs. rename y2 into be.  rename ys3 into bes.
+  destruct (B.value_dec be) as [[be_v ?] | ?].
+
+  + eexists. split. right. split. reflexivity.
+    * admit. (* metric *)
+    * eapply IInValue with (depth := 0)
+        (apat := fun v => S.MkConstr _ (_ ++ v :: _))
+        (bpat := fun v => S.MkConstr _ (_ ++ v :: _));
+        simpl; eauto using I_expr_expr_value.
+      -- i_ctor. i_lem Forall2_app.
+      -- simpl. reflexivity.
+
+  + (* Left and right are both values.  Proceed in lockstep. *)
+    eexists. split. left. i_lem B.SConstrStep.
+    i_ctor. i_ctor.
+
+(* SConstrStep - IInValue *)
+- eexists. split. right. split. reflexivity.
+  + admit. (* metric *)
+  + eapply IInValue with (depth := S depth); simpl; eauto.
+
+(* SConstrDone *)
+- eexists. split. left. i_lem B.SConstrDone.
+  + i_ctor. eapply I_expr_expr_value'_list. i_lem Forall2_map_l.
+  + i_lem I_run_cont.
+
+(* SConstrDone - IInValue *)
+- destruct depth as [ | depth' ].
+
+  + (* Depth is zero.  Left pops a continuation, returning to correspondence
+       with the right. *)
+    simpl in *.
+    inject_some.
+    on (B.expr_value (S.MkConstr _ _) _), invc.
+    fwd eapply expr_value_eq_list; eauto. subst.
+    on (S.run_cont _ _ = _), fun H => (rewrite H; clear H).
+
+    eexists. split. right. split. reflexivity.
+    * admit. (* metric *)
+    * i_ctor. on _, eapply_. i_ctor.
+
+  + (* Depth is nonzero.  Left pops a continuation and remains in IInValue. *)
+    fwd eapply unroll_cont_ex as HH; eauto.  destruct HH as (ae_last' & ?).
+    destruct ak; try discriminate; simpl in *.
+    all: break_and; subst l0.
+
+    * eexists. split. right. split. reflexivity.
+      -- admit. (* metric *)
+      -- i_lem IInValue.
+         eapply unroll_cont_expr_value with (result := ae_last); eauto.
+         eapply MkConstr_expr_value, MkConstr_expr_value_2.
+
+    * eexists. split. right. split. reflexivity.
+      -- admit. (* metric *)
+      -- i_lem IInValue.
+         eapply unroll_cont_expr_value with (result := ae_last); eauto.
+         eapply MkClose_expr_value, MkConstr_expr_value_2.
+
+
+(* SCloseStep *)
+- on _, invc_using Forall2_3part_inv.
+  rename ys1 into bvs. rename y2 into be.  rename ys3 into bes.
+  destruct (B.value_dec be) as [[be_v ?] | ?].
+
+  + eexists. split. right. split. reflexivity.
+    * admit. (* metric *)
+    * eapply IInValue with (depth := 0)
+        (apat := fun v => S.MkClose _ (_ ++ v :: _))
+        (bpat := fun v => S.MkClose _ (_ ++ v :: _));
+        simpl; eauto using I_expr_expr_value.
+      -- i_ctor. i_lem Forall2_app.
+      -- simpl. reflexivity.
+
+  + (* Left and right are both values.  Proceed in lockstep. *)
+    eexists. split. left. i_lem B.SCloseStep.
+    i_ctor. i_ctor.
+
+(* SCloseStep - IInValue *)
+- eexists. split. right. split. reflexivity.
+  + admit. (* metric *)
+  + eapply IInValue with (depth := S depth); simpl; eauto.
+
+(* SCloseDone *)
+- eexists. split. left. i_lem B.SCloseDone.
+  + i_ctor. eapply I_expr_expr_value'_list. i_lem Forall2_map_l.
+  + i_lem I_run_cont.
+
+(* SCloseDone - IInValue *)
+- destruct depth as [ | depth' ].
+
+  + (* Depth is zero.  Left pops a continuation, returning to correspondence
+       with the right. *)
+    simpl in *.
+    inject_some.
+    on (B.expr_value (S.MkClose _ _) _), invc.
+    fwd eapply expr_value_eq_list; eauto. subst.
+    on (S.run_cont _ _ = _), fun H => (rewrite H; clear H).
+
+    eexists. split. right. split. reflexivity.
+    * admit. (* metric *)
+    * i_ctor. on _, eapply_. i_ctor.
+
+  + (* Depth is nonzero.  Left pops a continuation and remains in IInValue. *)
+    fwd eapply unroll_cont_ex as HH; eauto.  destruct HH as (ae_last' & ?).
+    destruct ak; try discriminate; simpl in *.
+    all: break_and; subst l0.
+
+    * eexists. split. right. split. reflexivity.
+      -- admit. (* metric *)
+      -- i_lem IInValue.
+         eapply unroll_cont_expr_value with (result := ae_last); eauto.
+         eapply MkConstr_expr_value, MkClose_expr_value_2.
+
+    * eexists. split. right. split. reflexivity.
+      -- admit. (* metric *)
+      -- i_lem IInValue.
+         eapply unroll_cont_expr_value with (result := ae_last); eauto.
+         eapply MkClose_expr_value, MkClose_expr_value_2.
+
+
+(* SElimTarget *)
+- destruct (B.value_dec btarget) as [[btarget_v ?] | ?].
+
+  + eexists. split. right. split. reflexivity.
+    * admit. (* metric *)
+    * eapply IInValue with (depth := 0)
+        (apat := fun v => S.Elim _ _ v)
+        (bpat := fun v => S.Elim _ _ v);
+        simpl; eauto using I_expr_expr_value.
+      -- i_ctor.
+      -- simpl. reflexivity.
+
+  + (* Left and right are both values.  Proceed in lockstep. *)
+    eexists. split. left. i_lem B.SElimTarget.
+    i_ctor. i_ctor.
+
+
+(* SEliminate *)
+- fwd eapply Forall2_nth_error_ex as HH; eauto.  destruct HH as (bcase & ? & ?).
+  on (I_expr (S.Value _) _), invc.
+  eexists. split. left. i_lem B.SEliminate.
+  i_ctor. i_lem I_unroll_elim. i_ctor.
+
+Admitted.
